compcert_new/x86/Asm.v
@@ -1256,7 +1256,7 @@ Definition after_external_regset (ge:genv)(vret: option val) (rs: regset) : opti
       | Some res => 
           Some ((set_pair (loc_external_result (ef_sig ef)) res rs) #PC <- (rs RA))
       | None => 
-          Some ( rs #PC <- (rs RA))
+          Some (rs#(IR RAX) <- Vundef #PC <- (rs RA))
      end
     | _ => None
    end
